add more tests for sha3

code/experimental/sha3/Hacl.SHA3.fst
@@ -86,3 +86,40 @@ val sha3_512:
      (ensures  fun h0 _ h1 -> modifies (loc_buffer output) h0 h1)
 let sha3_512 inputByteLen input output =
   keccak (size 576) (size 1024) inputByteLen input (u8 0x06) (size 64) output
+
+(* cSHAKE for Frodo *)
+val cshake128_frodo:
+     input_len:size_t
+  -> input:lbuffer uint8 (v input_len)
+  -> cstm:uint16
+  -> output_len:size_t
+  -> output:lbuffer uint8 (v output_len)
+  -> Stack unit
+    (requires fun h -> B.live h input /\ B.live h output /\ B.disjoint input output)
+    (ensures  fun h0 _ h1 -> modifies (loc_buffer output) h0 h1)
+let cshake128_frodo input_len input cstm output_len output =
+  push_frame ();
+  let s = create (size 25) (u64 0) in
+  s.(size 0) <- u64 0x10010001a801 |. (to_u64 cstm <<. u32 48);
+  state_permute s;
+  absorb s (size 168) input_len input (u8 0x04);
+  squeeze s (size 168) output_len output;
+  pop_frame ()
+
+val cshake256_frodo:
+    input_len:size_t
+  -> input:lbuffer uint8 (v input_len)
+  -> cstm:uint16
+  -> output_len:size_t
+  -> output:lbuffer uint8 (v output_len)
+  -> Stack unit
+    (requires fun h -> B.live h input /\ B.live h output /\ B.disjoint input output)
+    (ensures  fun h0 _ h1 -> modifies (loc_buffer output) h0 h1)
+let cshake256_frodo input_len input cstm output_len output =
+  push_frame ();
+  let s = create (size 25) (u64 0) in
+  s.(size 0) <- u64 0x100100018801 |. (to_u64 cstm <<. u32 48);
+  state_permute s;
+  absorb s (size 136) input_len input (u8 0x04);
+  squeeze s (size 136) output_len output;
+  pop_frame ()
